LambdaLab/System/Basic.lean
@@ -1,0 +1,6 @@
+
+structure TypeSystem where
+  Tm : Type
+  Ty : Type
+
+  HasType : Ctx Ty → Tm → Ty → Prop
